Blake3Test.lean
@@ -1,7 +1,7 @@
 import Blake3
 
 abbrev input : ByteArray := ⟨#[0]⟩
-abbrev expected_output_regular_hashing : ByteArray := ⟨#[
+abbrev expectedOutputRegularHashing : ByteArray := ⟨#[
    45,  58, 222, 223, 241,  27,  97, 241,
    76, 136, 110,  53, 175, 160,  54, 115,
   109, 205, 135, 167,  77,  39, 181, 193,
@@ -9,13 +9,13 @@ abbrev expected_output_regular_hashing : ByteArray := ⟨#[
 ]⟩
 
 -- Good pseudo-random key
-abbrev key : ByteArray := ⟨#[
+abbrev key : Blake3.Blake3Key := .ofBytes ⟨#[
      3, 123,  16, 175,  8, 196, 101, 134,
    144, 184, 221,  34, 25, 106, 122, 200,
    213,  14, 159, 189, 82, 166,  91, 107,
     33,  78,  26, 226, 89,  65, 188, 92
 ]⟩
-abbrev expected_output_keyed_hashing: ByteArray := ⟨#[
+abbrev expectedOutputKeyedHashing: ByteArray := ⟨#[
    145, 187, 220, 234, 206, 139, 205, 138,
    220, 103,  35,  65, 199,  96, 210,  18,
    145, 201, 131, 254,  79, 208, 229, 157,
@@ -24,16 +24,37 @@ abbrev expected_output_keyed_hashing: ByteArray := ⟨#[
 
 -- Context (with "bad" randomness)
 abbrev context : ByteArray := ⟨#[0, 1, 2, 3, 4, 5, 6, 7, 8, 9, 10, 11, 12, 13, 14, 15]⟩
-abbrev expected_output_derive_key_hashing: ByteArray := ⟨#[
+abbrev expectedOutputDeriveKeyHashing: ByteArray := ⟨#[
     34,  57,  22,  43, 164, 211,  65, 131,
     90,  55,  55,  92,  68,  90,  63, 136,
      3, 235,  52, 117, 143, 246, 158, 224,
-   178, 170, 234, 211, 148,  21,  97, 183]⟩
+   178, 170, 234, 211, 148,  21,  97, 183
+]⟩
+
+abbrev expectedOutputSponge : ByteArray := ⟨#[
+    21, 150, 121,  38, 177,  21,  33, 148, 213, 127,
+   208, 231, 200,  18,  46, 115, 244, 188, 245, 188,
+   176,  29,  43, 123, 135, 148, 132, 218,  45, 244,
+   127, 103, 178,  82, 145,  67,  43, 106, 204, 137,
+   154,  99, 175,   9, 196, 102, 126,  72,  27,  86
+]⟩
+
+def hashingFails :=
+  (Blake3.hash input).val.data != expectedOutputRegularHashing.data ||
+  (Blake3.hashKeyed input key).val.data != expectedOutputKeyedHashing.data ||
+  (Blake3.hashDeriveKey input context).val.data != expectedOutputDeriveKeyHashing.data
+
+def spongeFails :=
+  let sponge := Blake3.Sponge.init "ix 2025-01-01 16:18:03 content-addressing v1"
+  let sponge := sponge.absorb ⟨#[1]⟩
+  let sponge := sponge.absorb ⟨#[2]⟩
+  let sponge := sponge.absorb ⟨#[3]⟩
+  let sponge := sponge.absorb ⟨#[4, 5]⟩
+  let output := sponge.squeeze 50
+  output.val.data != expectedOutputSponge.data
 
 def main : IO UInt32 := do
   println! s!"BLAKE3 version: {Blake3.version}"
-  if (Blake3.hash input).val.data != expected_output_regular_hashing.data ||
-     (Blake3.hashKeyed input key).val.data != expected_output_keyed_hashing.data ||
-     (Blake3.hashDeriveKey input context).val.data != expected_output_derive_key_hashing.data
+  if hashingFails || spongeFails
     then IO.eprintln "BLAKE3 test failed";    return 1
     else IO.println  "BLAKE3 test succeeded"; return 0
